\message{ !name(Assignment_1.tex)}\documentclass[11pt]{article}
\usepackage[]{ragged2e}
\usepackage{fancyhdr,amsmath,amsthm,amssymb,bbm}
\usepackage[utf8]{inputenc}

\usepackage[letterpaper,left=25mm,right=25mm]{geometry}

\setlength{\parskip}{1em}
\setlength{\parindent}{0em}

\newcommand{\Z}{\mathbb{Z}}
\newcommand{\R}{\mathbb{R}}
\newcommand{\Q}{\mathbb{Q}}
\newcommand{\C}{\mathbb{C}}

\DeclareMathOperator{\Ima}{Im}

\linespread{1.25}
\pagestyle{fancy}
\fancyhf{}
\lhead{PHYS 359 $|$ Assignment 1}

\rhead{Dilraj Ghuman $|$ 20564228}

\begin{document}

\message{ !name(Assignment_1.tex) !offset(-3) }


\textbf{Problem 1}

\textbf{(a)} To show this relation, we simply do a direct computation.

$$\lim_{a \to 1} \int_{0}^{\infty} \left(-1 \frac{\partial}{\partial a} \right)^{N}e^{-ax}dx = \lim_{a \to 1} \int_{0}^{\infty} (-1)^{N} \left(\frac{\partial}{\partial a} \right)^{N}e^{-ax}dx$$
$$ = \lim_{a \to 1} \int_{0}^{\infty} (-1)^{N}(-1)^{N} x^{N}e^{-ax}dx$$
$$ = \lim_{a \to 1} \int_{0}^{\infty} x^{N}e^{-ax}dx$$
$$ = \int_{0}^{\infty} x^{N}e^{-x}dx$$

\textbf{(b)} This relation can be shown by evaluating the integral first.

$$\lim_{a \to 1} \left(-1 \frac{\partial}{\partial a} \right)^{N} \int_{0}^{\infty}e^{-ax}dx = \lim_{a \to 1} \left(-1\frac{\partial}{\partial a}\right)^{N} \frac{1}{a}$$
$$ = \lim_{a\to 1} (-1)^{N} \prod_{i=1}^{N}(-1)ia^{-(i+1)}$$
$$ = \lim_{a\to 1}(-1)^{N}(-1)^{N}N! \prod_{i=1}^{N} a^{-(i+1)} = N!$$

\textbf{(c)} We define the substitution. Thus, let $x = N + y\sqrt{N}$, then, $dx = dy\sqrt{N}$. Now to get the bounds, as $x \to 0$ we see $y \to -\sqrt{N}$, and as $x \to \infty$, $y \to \infty$. Substituting these in we get,

$$\int_{0}^{\infty} x^{N}e^{-x}dx = \int_{-\sqrt{N}}^{\infty} (N+y\sqrt{N})^{N}e^{-(N+y\sqrt{N})}\sqrt{N}dy$$
$$ = \int_{-\sqrt{N}}^{\infty} N^{N}\left(1+\frac{y\sqrt{N}}{N}\right)^{N}e^{-(N+y\sqrt{N})}\sqrt{N}dy$$
$$ =N^{N}\sqrt{N}e^{-N} \int_{-\sqrt{N}}^{\infty} \left(1+\frac{y\sqrt{N}}{N}\right)^{N}e^{-y\sqrt{N}}dy$$

We now use our approximation by replacing $1+\frac{y\sqrt{N}}{N}$ with $e^{ln(1+\frac{y\sqrt{N}}{N})}$. Thus,

$$N^{N}\sqrt{N}e^{-N} \int_{-\sqrt{N}}^{\infty} \left(1+\frac{y\sqrt{N}}{N}\right)^{N}e^{-y\sqrt{N}}dy= N^{N}\sqrt{N}e^{-N} \int_{-\sqrt{N}}^{\infty} \left(e^{\frac{y\sqrt{N}}{N} - \frac{y^{2}}{N}}\right)^{N}e^{-y\sqrt{N}}dy$$
$$ = $$





\message{ !name(Assignment_1.tex) !offset(-5) }

\end{document}
